systematic use of empty_locals

theories/RealizabilitySemantics.v
@@ -80,8 +80,6 @@ Section Realizability.
 
   Open Scope bs. 
 
-  Definition empty_locals : Ident.Map.t := fun _ => fail "notfound".
-
   Close Scope bs. 
 
   Section Values. 
